tests/elab/vcgenForallRhs.lean
@@ -35,7 +35,7 @@ axiom wp_add : ∀ {l r : Lang} {Φ : Value → Prop},
 instance instWP_Lang : WP Lang Value Prop EStack⟨⟩ where
   wpTrans l := ⟨fun Φ _ => wp l Φ⟩
   wp_trans_monotone x := by
-    simp [PredTrans.Monotone, Lean.Order.PartialOrder.rel]
+    simp [PredTrans.monotone, Lean.Order.PartialOrder.rel]
     intros; apply wp_mono <;> trivial
 
 @[spec]
@@ -82,7 +82,7 @@ axiom wpS_add : ∀ {l r} {Φ : ValueS → Nat → Prop} {s : Nat},
 instance instWP_LangS : WP LangS ValueS (Nat → Prop) EStack⟨⟩ where
   wpTrans l := ⟨fun Φ _ => wpS l Φ⟩
   wp_trans_monotone x := by
-    simp [PredTrans.Monotone, Lean.Order.PartialOrder.rel]
+    simp [PredTrans.monotone, Lean.Order.PartialOrder.rel]
     intros; apply wpS_mono <;> trivial
 
 @[spec]
