tests/elab/vcgenMVarProgram.lean
@@ -41,7 +41,7 @@ axiom wp_bnd : ∀ {k : Nat → Lang} {Φ : Value → Prop},
 instance instWP_Lang : WP Lang Value Prop EStack⟨⟩ where
   wpTrans l := ⟨fun Φ _ => wp l Φ⟩
   wp_trans_monotone x := by
-    simp [PredTrans.Monotone, Lean.Order.PartialOrder.rel]
+    simp [PredTrans.monotone, Lean.Order.PartialOrder.rel]
     intros; apply wp_mono <;> trivial
 
 @[spec]
